Prove run-length invertible and bounded

RunLength.v
@@ -3,68 +3,141 @@ Import ListNotations.
 Require Import Coq.Init.Nat.
 Require Import Omega.
 Require Import Coq.Bool.Bool.
+Require Import Recdef.
 
 Require Import VST.fcf.EqDec.
 
-Open Scope eq_scope.
-Open Scope bool_scope.
-
 Section RunLength.
 
-  Generalizable Variable A.
-  Context `{EqDec A}.
+  Open Scope bool_scope.
+  Open Scope nat_scope.
+  Open Scope eq_scope.
 
-  Definition run_length_cons (maxRun : nat) (x: A) (l: list (A * nat)) :=
+  Generalizable Variable A.
+  Context `{ED : EqDec A}.
+
+  (* maxRun is the maximum length of a run. Useful if we want to
+       later encode the run-length encoded list in some fixed-size
+       binary representation, so we have a limit on the largest
+       representable number. *)
+  Variable maxRun : nat.
+  Hypothesis HMaxRunPos : maxRun > 0.
+
+  (* Add one element to a run-length encoded list l. *)
+  Definition run_length_cons (x: A) (l: list (A * nat)) :=
     match l with
     | nil => [(x,1)]
-    | (y,count)::tl => if (x ?= y) && (ltb count maxRun)
-                      then (x, count+1)::tl
-                      else (x,1) :: (y, count) :: tl
+    | (y,count)::tl =>
+      if (x ?= y) && (count <? maxRun)
+      then (x, Nat.succ count) :: tl
+      else (x,1) :: (y, count) :: tl
     end.
 
-  Definition run_length_encode maxRun :=
-    List.fold_right (run_length_cons maxRun) [].
+  (* Run length encode an entire list. *)
+  Definition run_length_encode :=
+    List.fold_right run_length_cons [].
 
-  Definition run_length_cons_inverse (x: (A * nat)) (l: list A) :=
-    match x with
-    | (el, count) => List.repeat el count ++ l
-    end.
+  Lemma run_length_cons_cases : forall x l
+                                  (P: A -> list (A * nat) -> list (A * nat) -> Prop),
+      P x [] [(x, 1)] ->
+      (forall hd count tl, x = hd -> count < maxRun ->
+                      P x ((hd,count)::tl) ((hd, Nat.succ count)::tl)) ->
+      (forall hd count tl, x = hd -> count >= maxRun ->
+                      P x ((hd,count)::tl) ((x,1)::(hd,count)::tl)) ->
+      (forall hd count tl, x <> hd -> P x ((hd,count)::tl) ((x,1)::(hd,count)::tl)) ->
+      P x l (run_length_cons x l).
+  Proof.
+    intros x l P HBase HEq HOver HNew.
+    induction l as [| p tl].
+    - apply HBase.
+    - destruct p as [hd count].
+      destruct (EqDec_dec _ x hd) as [Eq | Neq].
+      + simpl. rewrite (proj2 (eqb_leibniz _ _) Eq).
+        destruct (le_lt_dec maxRun count) as [ Ge | Lt ].
+        * assert (Ge': count >= maxRun) by omega.
+          rewrite (proj2 (Nat.ltb_ge _ _) Ge'). simpl.
+          apply HOver; auto.
+        * rewrite (proj2 (Nat.ltb_lt _ _) Lt). simpl.
+          subst x. apply HEq; auto.
+      + simpl. rewrite (proj2 (eqb_false_iff _ _ _) Neq).
+        rewrite andb_false_l.
+        apply HNew; auto.
+  Qed.
 
-  Definition run_length_decode (l : list (A * nat)) :=
-    List.fold_right run_length_cons_inverse [] l.
-
-  Definition run_bounded maxRun (l: list (A * nat)) :=
+  Definition run_bounded (l: list (A * nat)) :=
     Forall (fun x => x <= maxRun) (map snd l).
 
-  Theorem run_length_cons_bounded : forall maxRun x l,
-      maxRun > 0 ->
-      run_bounded maxRun l -> run_bounded maxRun (run_length_cons maxRun x l).
+  Lemma run_length_cons_bounded : forall x l,
+      run_bounded l -> run_bounded (run_length_cons x l).
   Proof.
-    intros. destruct l.
-    - (* empty list *)
-      unfold run_bounded. simpl.
-      econstructor. omega. econstructor.
-    - (* nonempty list *)
-      destruct p. simpl.
-      destruct (EqDec_dec H x a).
-      + (* x equal to head of list *)
-        destruct (eqb_leibniz x a) as [_ L].
-        specialize (L e). rewrite L. simpl.
-        destruct (Nat.ltb_spec n maxRun).
-        * (* n < maxRun *)
-          unfold run_bounded in *. simpl.
-          econstructor. omega.
-          inversion H1. auto.
-        * (* n >= maxRun *)
-          unfold run_bounded in *. simpl.
-          repeat (econstructor; try omega; auto).
-      + (* x is new *)
-        destruct (eqb_false_iff H x a) as [_ L].
-        specialize (L n0). rewrite L. simpl.
-        repeat (econstructor; try omega; auto).
+    intros x l.
+    apply run_length_cons_cases;
+      try (intros hd count tl HEq HLT HInd);
+      simpl; try (inversion HInd; subst); econstructor; auto; simpl; try omega.
+  Qed.
+
+  Theorem run_length_bounded : forall l,
+      run_bounded (run_length_encode l).
+  Proof.
+    induction l.
+    - econstructor.
+    - unfold run_length_encode. simpl.
+      apply run_length_cons_bounded; auto.
+  Qed.
+
+  (* We define a measure that will decrease on each recursive call to
+     run_length_decode, so that we can prove that it terminates. To
+     that end, we measure the cons cell itself as 1 so that the
+     measure decreases when we remove a cons cell with a 0 run.*)
+  Fixpoint run_length_measure (l : list (A * nat)) :=
+    match l with
+    | [] => 0
+    | (_,count)::tl =>
+      if count ?= 0
+      then 1 + run_length_measure tl
+      else 1 + count + run_length_measure tl
+    end.
+
+  Function run_length_decode (l : list (A * nat)) { measure run_length_measure l } :=
+    match l with
+    | [] => []
+    | (x,count)::tl =>
+      if 0 <? count
+      then x :: run_length_decode ((x, Nat.pred count) :: tl)
+      else run_length_decode tl
+    end.
+  Proof.
+    - intros l p tl x count HP HL HLT. simpl.
+      destruct (Nat.eq_dec 1 count) as [Eq | NEq].
+      + subst. simpl. omega.
+      + apply Nat.ltb_lt in HLT.
+        assert (HLT': 0 < Nat.pred count) by omega.
+        rewrite (proj2 (Nat.leb_gt _ _) HLT').
+        rewrite (proj2 (Nat.leb_gt _ _) HLT). simpl.
+        omega.
+    - intros l p tl x count HP HL HLT. simpl.
+      rewrite Nat.ltb_antisym in HLT.
+      rewrite (proj1 (negb_false_iff _) HLT).
+      simpl. omega.
+  Defined.
+
+  Lemma run_length_cons_invert : forall x l,
+      run_length_decode (run_length_cons x l) = x :: run_length_decode l.
+  Proof.
+    intros x l.
+    apply run_length_cons_cases;
+      intros; simpl;
+        do 2 (try (rewrite run_length_decode_equation);
+              simpl; subst; try reflexivity).
+  Qed.
+
+  Theorem run_length_invert : forall l,
+    run_length_decode (run_length_encode l) = l.
+  Proof.
+    induction l as [| hd tl].
+    - rewrite run_length_decode_equation. reflexivity.
+    - simpl. rewrite run_length_cons_invert.
+      f_equal. apply IHtl.
   Qed.
 
 End RunLength.
-
-Compute run_length_encode 2 [1; 1; 1; 2; 2; 3; 2; 1].
-Compute run_length_decode (run_length_encode 2 [1; 1; 1; 2; 2; 3; 2; 1]).
